io/IIO.Behavior.fst
@@ -17,22 +17,20 @@ assume val __reify_IIOwp (#a:Type) (#wp:Hist.hist a) (#fl:tflag) ($f:unit -> IIO
    'backward predicate transformer 2.3.4' and the 
    'pre-/postcondition transformer 2.3.2' to obtain
    the 'set' of traces produces by the whole program. *)
-val beh_giio : (list string -> GTot (dm_giio int AllActions trivial_hist)) -> trace_property #event
+val beh_giio : dm_giio int AllActions trivial_hist -> trace_property #event
 let beh_giio ws tr =
   match tr with
-  | Infinite_trace _ _ -> False
-  | Finite_trace args lt res -> 
+  | Infinite_trace _ -> False
+  | Finite_trace lt res -> 
    (* We verify specs of whole programs, thus, instead of having
       properties forall histories, we can specialize it for the
       empty history *)
-    forall p. dm_giio_theta (ws args) p [] ==> p lt res
+    forall p. dm_giio_theta ws p [] ==> p lt res
 
-val _beh : (list string -> IIO int AllActions (fun _ -> True) (fun _ _ _ -> True)) -> trace_property #event
+val _beh : (unit -> IIO int AllActions (fun _ -> True) (fun _ _ _ -> True)) -> trace_property #event
 let _beh ws =
-  beh_giio (fun args -> 
-    let ws' : unit -> IIO int AllActions (fun _ -> True) (fun _ _ _ -> True) = (fun () -> ws args) in
-    __reify_IIOwp (fun () -> ws args))
+  beh_giio (__reify_IIOwp ws) 
 
 irreducible
-val beh : (list string -> IIO int AllActions (fun _ -> True) (fun _ _ _ -> True)) ^-> trace_property #event
+val beh : (unit -> IIO int AllActions (fun _ -> True) (fun _ _ _ -> True)) ^-> trace_property #event
 let beh = on_domain _ (fun ws -> _beh ws)
